Clap/Lang/FB/assert.lean
@@ -1,10 +1,20 @@
 import Clap.Lang.FB.FB
 import Clap.Lang.FB.not
+import Clap.Lang.FB.and
 
 namespace Clap.Edsl.Lang.FB
 
 def assert {p : ℕ} [Fact (p ≥ 2)] (a : FB p) : Edsl.CircuitStateM p Unit := do
   Edsl.eq0 (not a)
+
+def assertBool {p : ℕ} [Fact (p ≥ 2)] (a : FB p) : Edsl.CircuitStateM p Unit := do
+  Edsl.eq0 (and a a.not)
+
+def conditionallyAssert {p : ℕ} [Fact (p ≥ 2)] (antecedent consequent : FB p) :
+  Edsl.CircuitStateM p Unit
+:= do
+  -- a → c ≡ ¬(a ∧ ¬c)
+  Edsl.eq0 (and antecedent consequent.not)
 
 namespace assert
 
@@ -24,10 +34,27 @@ def matchesUnaryPredicatePure
     numAllocPost = numAlloc ∧
     varStorePost = varStore
 
-def spec (p : ℕ) [Fact (p ≥ 2)] : Prop := matchesUnaryPredicatePure p (·) FB.assert
+def matchesBinaryPredicatePure
+  (p : ℕ)
+  (spec_function : Bool → Bool → Prop)
+  (function : FB p → FB p → Edsl.CircuitStateM p Unit)
+: Prop :=
+  ∀ (a b : FB p) varStore numAlloc,
+    a.isValid (varStore.get?) →
+    b.isValid (varStore.get?) →
+    let ⟨numAllocPost, varStorePost, constraints⟩ := Edsl.CircuitState.eval
+      ((function a b).run numAlloc).1.2
+      varStore
+      numAlloc
+    constraints = spec_function (a.toBool varStore.get?) (b.toBool varStore.get?) ∧
+    numAllocPost = numAlloc ∧
+    varStorePost = varStore
 
-lemma equiv (p : ℕ) [Fact (p ≥ 2)] :
-  spec p
+
+def assert_spec (p : ℕ) [Fact (p ≥ 2)] : Prop := matchesUnaryPredicatePure p (·) FB.assert
+
+lemma assert_equiv (p : ℕ) [Fact (p ≥ 2)] :
+  assert_spec p
 := by
   intro a varStore numAlloc h_isValid
   simp [
@@ -35,8 +62,38 @@ lemma equiv (p : ℕ) [Fact (p ≥ 2)] :
     FB.assert,
     h_isValid,
     not.equiv a,
-    ofBool.equiv
+    ofBool.equiv]
+
+def assertBool_spec (p : ℕ) [Fact (p ≥ 2)] : Prop :=
+  matchesUnaryPredicatePure p (Function.const Bool True) FB.assertBool
+
+lemma assertBool_equiv (p : ℕ) [Fact (p ≥ 2)] :
+  assertBool_spec p
+:= by
+  intro a varStore numAlloc h_isValid
+  simp [
+    Clap.monads,
+    FB.assertBool,
+    and.equiv a a.not _ h_isValid (not.not_isValid h_isValid)
   ]
+  simp_all [toBool, not.equiv a, ofBool.equiv]
+
+def conditionallyAssert_spec (p : ℕ) [Fact (p ≥ 2)] : Prop :=
+  matchesBinaryPredicatePure p (fun a c ↦ !(a && !c)) FB.conditionallyAssert
+
+lemma conditionallyAssert_equiv (p : ℕ) [Fact (p ≥ 2)] :
+  conditionallyAssert_spec p
+:= by
+  intro a c varStore numAlloc h_isValid_a h_isValid_c
+  simp [
+    Clap.monads,
+    FB.conditionallyAssert,
+    and.equiv a c.not _ h_isValid_a (not.not_isValid h_isValid_c),
+    ofBool.equiv,
+    ]
+  by_cases h₁ : a.toBool varStore.get? <;>
+  by_cases h₂ : c.toBool varStore.get? <;>
+  simp [h₁, h₂, not.not_toBool h_isValid_c]
 
 end assert
 
