Clap/Lang/FB/and.lean
@@ -1,0 +1,18 @@
+import Clap.Lang.FB.FB
+
+namespace Clap.Edsl.Lang.FB
+
+def and {p : ℕ} [Fact (p ≥ 2)] (a b : FB p) : FB p := a * b
+
+namespace and
+
+def spec (p : ℕ) [Fact (p ≥ 2)] : Prop :=
+  matchesBinaryFunction p (· && ·) FB.and
+
+lemma equiv {p : ℕ} [Fact (p ≥ 2)] : spec p := by
+  intro a varStore h_isValid
+  aesop (add simp [FB.and, toBool,isValid, beq_eq_false_iff_ne.mpr, FixedExp.eval])
+
+end and
+
+end Clap.Edsl.Lang.FB
