Clap/Lang/FB/xor.lean
@@ -1,0 +1,22 @@
+import Clap.Lang.FB.FB
+
+namespace Clap.Edsl.Lang.FB
+
+def xor {p : ℕ} [Fact (p ≥ 2)] (a b : FB p) : FB p := a + b - 2 * a * b
+
+namespace xor
+
+def spec (p : ℕ) [Fact (p ≥ 2)] : Prop :=
+  matchesBinaryFunction p (· ^^ ·) FB.xor
+
+lemma equiv {p : ℕ} [Fact (p ≥ 2)] : spec p := by
+  intro a varStore h_isValid h₁ h₂
+  aesop (add simp [
+    FB.xor, left_inv, right_inv, toBool, FB.false, isValid,
+    beq_eq_false_iff_ne.mpr, ofBool, FixedExp.eval
+  ])
+  norm_num
+
+end xor
+
+end Clap.Edsl.Lang.FB
